## 1.5运算性质
### 一、四则运算  
**引理1：`$\lim_{x\to a}f(x)=A\Leftrightarrow f(x)=A+\alpha\text{其中}\alpha\to0(x\to a)$`**  
证明："`$\Rightarrow$`"  
`$f(x) = A+f(x)-A$`  
`$\forall\epsilon>0,\because\lim_{x\to a}f(x)=A.$`  
`$\therefore\exists\delta>0.\text{当}0<|x-a|<\delta\text{时}.|f(x)-A|<\epsilon$`  
`$\text{令}\alpha = f(x)-A.f(x)=A+\alpha.$`  
`$\text{即}\forall\epsilon>0,\exists\delta>0,\text{当}0<|x-a|<\delta\text{时},|\alpha|<\epsilon$`  
`$\lim_{x\to a}\alpha=0.$`  
证明："`$\Leftarrow$`"  
`$\text{设}f(x)=A+\alpha\text{且}\alpha\to0(x\to a)$`  
`$\because\lim_{x\to a}\alpha=0.$`  
`$\therefore\forall\epsilon>0,\exists\delta>0.\text{当}0<|x-a|<\delta\text{时},|\alpha|<\epsilon$`  
`$\text{即}|f(x)-A|<\epsilon$`  
`$\therefore\lim_{x\to a}f(x)=A.$`  

**引理2:**  
①`$\alpha\to0,\beta\to0(x\to a)\Rightarrow\alpha\pm\beta\to0(x\to a)$`  
证明：  
`$\forall\epsilon>0.$`  
`$\because\lim_{x\to a}\alpha=0.$`  
`$\therefore\exists\delta_1>0,\text{当}0<|x-a|<\delta_1\text{时}$`  
`$|\alpha|<\epsilon\quad(*)$`  
`$\because\lim_{x\to a}\beta=0.$`  
`$\therefore\exists\delta_2>0,\text{当}0<|x-a|<\delta_2\text{时}$`  
`$|\beta|<\epsilon\quad(**)$`  
`$\text{取}\delta=min\{\delta_1,\delta_2\},$`  
`$\text{当}0<|x-a|<\delta\text{时},(*)(**)\text{皆成立}$`  
`$|\alpha\pm\beta|\leq|\alpha|+|\beta|<2\epsilon$`  
`$\therefore\lim_{x\to a}(\alpha\pm\beta)=0.$`  

②`$\alpha\to0(x\to a),|\beta|\leq M.\Rightarrow\alpha\beta\to0(x\to a)$`  
证明：  
`$\forall\epsilon>0.$`  
`$\because\lim_{x\to a}\alpha=0.$`  
`$\therefore\exists\delta>0,\text{当}0<|x-a|<\delta\text{时},|\alpha-0|<\epsilon.$`  
`$|\alpha\beta-0|\leq M|\alpha|<M\epsilon$`  
`$\lim_{x\to a}\alpha\beta=0.$`  

③`$\alpha\to0(x\to a),M=constant\Rightarrow M\alpha\to 0(x\to a)$`  

④`$\alpha\to0,\beta\to0(x\to a)\Rightarrow\alpha\beta\to0(x\to a).$`  
证明：  
`$\text{取}\epsilon=1.$`
`$\because\lim_{x\to a}\beta=0\therefore\exists\delta_1>0,\text{当}0<|x-a|<\delta_1\text{时}$`  
`$|\beta|<1\quad(*)$`  
`$\forall\epsilon>0.$`  
`$\because\lim_{x\to a}\alpha=0\therefore\exists\delta_2>0,\text{当}0<|x-a|<\delta_2\text{时}$`  
`$|\alpha|<\epsilon\quad(**)$`  
`$\text{取}\delta=min\{\delta_1,\delta_2\},\text{当}0<|x-a|<\delta\text{时},(*)(**)\text{皆成立}$`    
`$\therefore|\alpha\beta|=|\alpha||\beta|<\epsilon,\text{即}\lim_{x\to a}\alpha\beta=0.$`  

**Th1.设`$\lim f(x)=A.\lim g(x)=B.$`则：**  
**①`$\lim[f(x)\pm g(x)]=A\pm B$`**  
**②`$\lim f(x)g(x)=AB$`**  
**③`$\lim\frac{g(x)}{f(x)}=\frac{B}{A}(A\not=0)$`**  

①证明：  
`$\lim f(x)=A\Rightarrow f(x)=A+\alpha,\alpha\to0.$`  
`$\lim g(x)=B\Rightarrow g(x)=B+\beta,\beta\to0.$`  
`$f(x)\pm g(x)=(A\pm B)+(\alpha\pm\beta)$`  
`$\because\alpha\pm\beta\to0$`  
`$\therefore\lim[f(x)\pm g(x)]=A\pm B.$`  

②证明：  
`$\lim f(x)=A\Rightarrow f(x)=A+\alpha,\alpha\to0.$`  
`$\lim g(x)=B\Rightarrow g(x)=B+\beta,\beta\to0.$`  
`$f(x)g(x)=(A+\alpha)(B+\beta)=AB+A\beta+\alpha B+\alpha\beta$`  
`$\because A\beta\to0,\alpha B\to0,\alpha\beta\to0.\Rightarrow(A\beta+\alpha B+\alpha\beta)\to0$`  
`$\lim f(x)g(x)=AB.$`  

③证明：  
`$\text{设}A\not=0. (\text{研究}x\to a)$`  
`$\text{取}\epsilon=\frac{|A|}{2}>0.$`  
`$\because\lim_{x\to a}f(x)=A.$`  
`$\therefore\exists\delta_1>0.$`  
`$\text{当}0<|x-a|<\delta_1\text{时},|f(x)-A|<\frac{|A|}{2}$`  
`$\Rightarrow|f(x)|>\frac{|A|}{2}\quad(*)$`  
`$\because\lim_{x\to a}g(x)=B.$`  
`$\therefore\forall\epsilon>0.\exists\delta_2>0,\text{当}0<|x-a|<\delta_2\text{时},|g(x)-B|<\epsilon\quad(**)$`  
`$|\frac{g(x)}{f(x)}-\frac{B}{A}|=\frac{1}{|A|f(x)}|Ag(x)-Bf(x)|$`  
`$\text{取}\delta=min\{\delta_1,\delta_2\}.$`  
`$\text{当}0<|x-a|<\delta\text{时},(*)(**)\text{皆成立}.$`  
`$\text{当}0<|x-a|<\delta\text{时},|\frac{g(x)}{f(x)}-\frac{B}{A}|<\frac{2}{|A|^2}|Ag(x)-Bf(x)|\quad(***)$`  
`$\lim_{x\to a}f(x)=A\Rightarrow f(x)=A+\alpha,\alpha\to0(x\to a)$`  
`$\lim_{x\to a}g(x)=B\Rightarrow g(x)=B+\beta,\beta\to0(x\to a)$`  
`$Ag(x)-Bf(x)=A\beta-B\alpha\to0(x\to a)$`  
`$\therefore\lim_{x\to a}\frac{g(x)}{f(x)}=\frac{B}{A}$`  

③简化证明：  
`$\lim_{x\to a}f(x)=A.\lim_{x\to a}g(x)=B.$`  
`$f(x)=A+\alpha,\alpha\to 0(x\to a)$`  
`$g(x)=B+\beta,\beta\to0(x\to a)$`  
`$|\frac{g(x)}{f(x)}-\frac{B}{A}|=|\frac{B+\beta}{A+\alpha}-\frac{B}{A}|=\frac{1}{|A||f(x)|}|A\beta-B\alpha|$`  
`$\text{取}\epsilon=\frac{|A|}{2}>0.$`  
`$\because\lim_{x\to a}f(x)=A.$`  
`$\therefore\exists\delta_1>0.$`  
`$\text{当}0<|x-a|<\delta_1\text{时}.$`  
`$||f(x)|-|A||\leq|f(x)-A|<\frac{|A|}{2}\Rightarrow|f(x)|>\frac{|A|}{2}\quad(*)$`  
`$\forall\epsilon>0.$`  
`$\lim_{x\to a}(A\beta-B\alpha)=0.$`  
`$\because\exists\delta_2>0.$`  
`$\text{当}0<|x-a|<\delta_2\text{时}.$`  
`$|A\beta-B\alpha|<\epsilon\quad(**)$`  
`$\text{取}\delta=min\{\delta_1,\delta_2\},$`  
`$\text{当}0<|x-a|<\delta\text{时},(*)(**)\text{皆成立}$`  
`$|\frac{g(x)}{f(x)}-\frac{B}{A}|<\frac{2}{|A|^2}\epsilon$`  
`$\therefore\lim_{x\to a}\frac{g(x)}{f(x)}=\frac{B}{A}$`    

例1.`$\lim_{x\to2}(2x+3)$`  
解：  
`$$`
`$\begin{aligned}\lim_{x\to2}(2x+3)
  &=\lim_{x\to2}2x+\lim_{x\to2}3\\
  &=2\lim_{x\to2}x+3\\
  &=7\end{aligned}$`  
**note:**  
`$P(x)=a_0+a_1x+...+a_nx^n$`,则`$\lim_{x\to a}P(x)=P(a)$`  

例2.`$\lim_{x\to1}\frac{x^2+x-2}{x^2-1}$`  
解：  
`$\begin{aligned}\lim_{x\to1}\frac{x^2+x-2}{x^2-1}&=\lim_{x\to1}\frac{(x-1)(x+2)}{(x-1)(x+1)}\\&=\lim_{x\to1}\frac{x+2}{x+1}\\&=\frac{\lim_{x\to1}(x+2)}{\lim_{x\to1}(x+1)}\\&=\frac{3}{2}\end{aligned}$`  

例3.`$\lim_{x\to\infty}\frac{x^2-2x+4}{2x^2+x}$`  
解：  
`$\begin{aligned}\lim_{x\to\infty}\frac{x^2-2x+4}{2x^2+x}&=\lim_{x\to\infty}\frac{1-\frac{2}{x}+\frac{4}{x^2}}{2+\frac{1}{x}}\\&=\frac{\lim_{x\to\infty}1-\lim_{x\to\infty}\frac{2}{x}+\lim_{x\to\infty}\frac{4}{x^2}}{\lim_{x\to\infty}2+\lim_{x\to\infty}\frac{1}{x}}\\&=\frac{1}{2}\end{aligned}$`  

例4.`$\lim_{x\to\infty}\frac{x+1}{x^2+2}$`  
解：  
`$\begin{aligned}\lim_{x\to\infty}\frac{x+1}{x^2+2}&=\lim_{x\to\infty}\frac{\frac{1}{x}+\frac{1}{x^2}}{1+\frac{1}{x^2}}\\&=0\end{aligned}$`  
**note:**  
`$P(x)=a_nx^n+...+a_1x+a_0.$`  
`$Q(x)=b_mx^m+...+b_1x+b_0.$`  
`$\lim_{x\to\infty}\frac{P(x)}{Q(x)}\begin{cases}\frac{a_n}{b_m}&,m=n\\0&,m>n\\\infty&,m<n\end{cases}$`  

### 二、复合
**Th2.`$y=f(u), u=g(x),\text{若}\lim_{x\to x_0}g(x)=a,\lim_{u\to a}f(u)=A,\text{则}\lim_{x\to x_0}f[g(x)]=A.$`**  
证：  
`$\forall\epsilon>0.$`  
`$\because\lim_{u\to a}f(u)=A.$`  
`$\therefore\exists\eta>0,\text{当}0<|u-a|<\eta\text{时},$`  
`$|f(u)-A|<\epsilon\quad(*)$`  
`$\text{对}\eta>0,\because\lim_{x\to x_0}g(x)=a.$`  
`$\therefore\exists\delta>0,\text{当}0<|x-x_0|<\delta\text{时},$`  
`$0<|g(x)-a|<\eta\quad(**)$`  
`$\therefore\forall\epsilon>0.\exists\delta>0.$`  
`$\text{当}0<|x-x_0|<\delta\text{时},$`  
`$|f[g(x)]-A|<\epsilon$`  
`$\lim_{x\to x_0}f[g(x)]=A.$`  

例题：  
`$\begin{aligned}\lim_{x\to1}(\frac{1}{1-x}-\frac{3}{1-x^3})&=\lim_{x\to1}\frac{x^2+x+4}{x^3-1}\\&=\lim_{x\to1}\frac{(x-1)^2-3(x-1)}{x^3-1}\\&=\lim_{x\to1}\frac{x-1}{x^2+x+1}-\lim_{x\to1}\frac{3}{x^2+x+1}\\&=-1\end{aligned}$`

> 两个函数趋向`$x_0$`，一个有极限，一个没有极限，其函数之和没有极限。  
证明：（反证法）  
`$\text{若}\lim_{x\to x_0}(f+g)=C.$`  
`$\because\lim_{x\to x_0}=A.$`  
`$\lim_{x\to x_0}[(f+g)-f]=C-A.$`  
`$\Rightarrow\lim_{x\to x_0}g=C-A.\text{矛盾}$`  

> 两个函数趋向`$x_0$`都没有极限，其函数之和可能有极限。  
`$\begin{aligned}\lim_{x\to1}(\frac{1}{1-x}-\frac{3}{1-x^3})&=-1\end{aligned}$`  

> 两个函数趋向`$x_0$`，一个有极限，一个没有极限，其函数之积可能有极限。