## 1.6存在性质
**准则一：（夹逼定理）**  
**case1.数列型**  
`$\begin{cases}a_n\leq b_n\leq c_n\\\lim_{n\to\infty}a_n=\lim_{n\to\infty}c_n=A\end{cases}\Rightarrow\lim_{n\to\infty}b_n=A.$`  
证：  
`$\forall\epsilon>0.$`  
`$\because\lim_{n\to\infty}a_n=A.$`  
`$\therefore\exists N_1>0,\text{当}n>N_1\text{时},$`  
`$|a_n-A|<\epsilon.\Leftrightarrow A-\epsilon<a_n<A+\epsilon\quad(*)$`  
`$\because\lim_{n\to\infty}c_n=A$`  
`$\therefore\exists N_2>0,\text{当}n >N_2\text{时},$`  
`$|c_n-A|<\epsilon\Leftrightarrow A-\epsilon<c_n<A+\epsilon\quad(**)$`  
`$\text{取}N=max\{N_1,N_2\},\text{当}n>N\text{时},(*)(**)\text{皆成立}.$`  
`$A-\epsilon<a_n\leq b_n\leq c_n<A+\epsilon\Rightarrow A-\epsilon<b_n<A+\epsilon\Leftrightarrow|b_n-A|<\epsilon$`  
`$\text{即}\forall\epsilon>0,\exists N>0,\text{当}n>N\text{时},|b_n-A|<\epsilon.$`  
`$\therefore\lim_{n\to\infty}b_n=A.$`  

例1.`$\lim_{n\to\infty}(\frac{1}{n^2+1}+\frac{2}{n^2+2}+...+\frac{n}{n^2+n})$`  
解：  
`$\because\frac{1+2+...+n}{n^2+n}\leq\frac{1}{n^2+1}+\frac{2}{n^2+2}+...+\frac{n}{n^2+n}\leq\frac{1+2+...+n}{n^2+1}$`  
`$\text{即}\frac{1}{2}\leq\frac{1}{n^2+1}+\frac{2}{n^2+2}+...+\frac{n}{n^2+n}\leq\frac{1}{2}\frac{n^2+n}{n^2+1}.$`  
`$\because\begin{cases}\lim_{n\to\infty}\frac{1}{2}=\frac{1}{2}\\\lim_{n\to\infty}\frac{1}{2}\frac{n^2+n}{n^2+1}=\frac{1}{2}\lim_{n\to\infty}\frac{1+\frac{1}{n}}{1+\frac{1}{n^2}}=\frac{1}{2}\end{cases}$`  
`$\therefore\lim_{n\to\infty}(\frac{1}{n^2+1}+\frac{2}{n^2+2}+...+\frac{n}{n^2+n})=\frac{1}{2}$`  

**case2.函数型**
`$\begin{cases}f(x)\leq g(x)\leq h(x)\\\lim f(x)=\lim h(x)=A\end{cases}\Rightarrow\lim g(x)=A.$`  
证明：（`$x\to a$`）  
`$\text{设}\begin{cases}f(x)\leq g(x)\leq h(x)\\\lim_{x\to a} f(x)=\lim_{x\to a}h(x)=A\end{cases}$`  
`$\forall\epsilon>0.$`  
`$\because\lim_{x\to a}f(x)=A.$`  
`$\therefore\exists\delta_1>0.\text{当}0<|x-a|<\delta_1\text{时},$`  
`$|f(x)-A|<\epsilon\Leftrightarrow A-\epsilon<f(x)<A+\epsilon\quad(*)$`  
`$\because\lim_{x\to a}h(x)=A.$`  
`$\therefore\exists\delta_2>0.\text{当}0<|x-a|<\delta_2\text{时},$`  
`$|h(x)-A|<\epsilon\Leftrightarrow A-\epsilon<h(x)<A+\epsilon\quad(**)$`    
`$\text{取}\delta=min\{\delta_1,\delta_2\}$`  
`$\text{当}0<|x-a|<\delta\text{时},(*)(**)\text{皆成立}$`  
`$A-\epsilon<f(x)\leq g(x)\leq h(x)<A+\epsilon$`  
`$\Rightarrow A-\epsilon<g(x)<A+\epsilon$`  
`$\Rightarrow|g(x)-A|<\epsilon$`  
`$\therefore\lim_{x\to a}g(x)=A.$`  

`$0<x<\frac{\pi}{2}$`
![image](https://img-blog.csdnimg.cn/20190212202652145.png?x-oss-process=image/watermark,type_ZmFuZ3poZW5naGVpdGk,shadow_10,text_aHR0cHM6Ly9ibG9nLmNzZG4ubmV0L3dlaXhpbl8zOTk4NjE4Nw==,size_16,color_FFFFFF,t_70)  
`$S_{\Delta AOB}=\frac{1}{2}\sin x.$`  
`$S_{\text{扇}AOB}=\frac{1}{2}x.$`  
`$S_{Rt AOC}=\frac{1}{2}\tan x.$`  
`$\frac{1}{2}\sin x<\frac{1}{2}x<\frac{1}{2}\tan x.\Leftrightarrow 1<\frac{x}{sinx}<\frac{1}{\cos x}.$`  
`$0 < 1-\cos x=2\sin^2\frac{x}{2}<2(\frac{x}{2})^2=\frac{1}{2}x^2$`  
`$\because\lim_{x\to0^+}0=0.$`  
`$\lim_{x\to0^+}\frac{1}{2}x^2 = 0.$`  
`$\therefore\lim_{x\to0^+}(1-\cos x)=0.$`  
`$\Rightarrow\lim_{x\to0^+}\cos x = 1.$`  
`$\because1<\frac{x}{sinx}<\frac{1}{\cos x}.$`  
`$\because\lim_{x\to0^+}1=1.$`  
`$\lim_{x\to0^+}\frac{1}{\cos x}=\frac{1}{\lim_{x\to0^+}\cos x}=1.$`  
`$\lim_{x\to0^+}\frac{x}{\sin x}=1.$`  
`$\frac{x}{\sin x}\text{为偶函数.}$`  
`$\therefore\lim_{x\to0^-}\frac{x}{\sin x}=1.$`  

**(重要极限I)：`$\lim_{\Delta\to0}\frac{\sin\Delta}{\Delta}=1.$`**  

**准则二：单调有界的数列必有极限**  
**Case1.`$\{a_n\}\uparrow\begin{cases}\text{无上界}\Rightarrow\lim_{n\to\infty}a_n=+\infty\\\text{有上界}.\exists M,a_n\leq M.\Rightarrow\lim_{n\to\infty}a_n\text{存在}\end{cases}$`**  
**Case2.`$\{a_n\}\downarrow\begin{cases}\text{无下界}\Rightarrow\lim_{n\to\infty}a_n=-\infty\\\text{有下界}.\exists M,a_n\geq M.\Rightarrow\lim_{n\to\infty}a_n\text{存在}\end{cases}$`**  

例1.`$a_1=\sqrt{2}, a_2=\sqrt{2+\sqrt{2}}, a_3=\sqrt{2+\sqrt{2+\sqrt{2}}},..., \text{证明:}\lim_{n\to\infty}a_n\text{存在，求之。}$`  
证：  
`$a_{n+1}=\sqrt{2+a_n}.\Rightarrow\{a_n\}\text{显然单调递增}.$`  
现证`$a_n\leq2.$`  
`$a_1=\sqrt{2}\leq2.$`  
`$\text{设}a_k\leq 2.$`  
`$a_{k+1}=\sqrt{2+a_k}\leq\sqrt{2+2}=2.$`  
`$\forall n,\text{有}a_n\leq2.$`  
`$\therefore\lim_{n\to\infty}a_n\text{存在}.$`  
`$\text{令}\lim_{n\to\infty}a_n = A.$`  
`$a_{n+1}=\sqrt{2+a_n}\Rightarrow A=\sqrt{2+A}.$`  
`$\Rightarrow A^2-A-2=0.$`  
`$\Rightarrow A=-1\text{(舍去)},A =2.$`  

例2.`$a_1=2,a_{n+1}=\frac{1}{2}(a_n+\frac{1}{a_n}),\text{证明：}\lim_{n\to\infty}a_n\text{存在}.$`  
证：  
> `$x+\frac{1}{x}\geq2.$`  

`$a_{n+1}=\frac{1}{2}(a_n+\frac{1}{a_n})\geq1.$`  
`$\forall n,a_n\geq1.$`  
`$\begin{aligned}a_{n+1}-a_n&=\frac{1}{2}(a_n+\frac{1}{a_n})-a_n\\&=\frac{1-a_n^2}{2a_n}\leq0\end{aligned}$`    
`$\Rightarrow a_{n+1}\leq a_n.$`  
`$\Rightarrow \{a_n\}\downarrow.$`  
`$\therefore\lim_{n\to\infty}a_n\text{存在}$`

例3.`$a_n=(1+\frac{1}{n})^n.$`  
解：  
`$\begin{aligned}a_n&=(1+\frac{1}{n})^n\\&=C^0_n+C^1_n\frac{1}{n}+C^2_n\frac{1}{n^2}+...+C^n_n\frac{1}{n^n}\\&=1+1+\frac{1}{2!}\frac{n(n-1)}{n^2}+...+\frac{1}{n!}\frac{n(n-1)(n-2)...2*1}{n^n}\\&=1+1+\frac{1}{2!}(1-\frac{1}{n})+...+\frac{1}{n!}(1-\frac{1}{n})...(1-\frac{n-1}{n})\end{aligned}$`  

`$\begin{aligned}a_{n+1}&=(1+\frac{1}{n+1})^{n+1}\\&=C^0_{n+1}+C^1_{n+1}\frac{1}{n+1}+C^2_{n+1}\frac{1}{(n+1)^2}+...+C^{n+1}_{n+1}\frac{1}{(n+1)^{n+1}}\\&=1+1+\frac{1}{2!}\frac{(n+1)n}{(n+1)^2}+...+\frac{1}{(n+1)!}\frac{(n+1)n(n-1)...2*1}{(n+1)^{n+1}}\\&=1+1+\frac{1}{2!}(1-\frac{1}{n+1})+...+\frac{1}{n!}(1-\frac{1}{n+1})...(1-\frac{n-1}{n+1})+\frac{1}{(n+1)^{n+1}}\end{aligned}$`  
`$\Rightarrow a_{n+1}>a_n\Rightarrow\{a_n\}\uparrow$`  
`$\because\begin{aligned}a_n&\leq1+1+\frac{1}{2!}+\frac{1}{3!}+...+\frac{1}{n!}\\&\leq1+1+\frac{1}{1*2}+\frac{1}{2*3}+...+\frac{1}{n(n-1)}\\&\leq3-\frac{1}{n}\leq3.\end{aligned}$`  
`$\because\begin{cases}\{a_n\}\uparrow\\a_n\leq3\end{cases}$`  
`$\lim_{n\to\infty}(1+\frac{1}{n})^n\text{存在}.$`  

**(重要极限II)：**  
**①`$\lim_{n\to\infty}(1+\frac{1}{n})^n=e.$`**    
**②`$\lim_{n\to\infty}(1+\frac{1}{x})^x=e.$`**  
**③`$\lim_{\Delta\to 0}(1+\Delta)^{\frac{1}{\Delta}}=e.$`**

例1.`$\lim_{n\to\infty}\frac{(n+1)^{n+1}}{n^n}\sin\frac{1}{n}$`  
解：  
`$\begin{aligned}\lim_{n\to\infty}\frac{(n+1)^{n+1}}{n^n}\sin\frac{1}{n}&=\lim_{n\to\infty}(\frac{n+1}{n})^{(n+1)}\frac{\sin\frac{1}{n}}{\frac{1}{n}}\\&=\lim_{n\to\infty}(1+\frac{1}{n})^n*(\frac{n+1}{n})*\frac{\sin\frac{1}{n}}{\frac{1}{n}}\\&=e\end{aligned}$`

例2.`$\lim_{x\to\infty}(1-\frac{1}{x})^{2x}.$`  
解：  
`$\begin{aligned}\lim_{x\to\infty}(1-\frac{1}{x})^{2x}&=\{[1+(-\frac{1}{x})]^{-x}\}^{-2}\\&=e^{-2}\end{aligned}$`  

例3.`$\lim_{x\to0}(1-2x)^\frac{1}{x}.$`  
解：  
`$\begin{aligned}\lim_{x\to0}(1-2x)^\frac{1}{x}&=\lim_{x\to0}(1+(-2x))^{(-\frac{1}{2x})*(-2)}\\&=e^{-2}\end{aligned}$`  

例4.`$\lim_{n\to\infty}(\sum^n_{k =1}\frac{1}{k(k+1)})^n$`  
解：  
`$\begin{aligned}\lim_{n\to\infty}(\sum^n_{k =1}\frac{1}{k(k+1)})^n&=\lim_{n\to\infty}(\sum^n_{k=1}(\frac{1}{k}-\frac{1}{k+1})^n\\&=\lim_{n\to\infty}(1-\frac{1}{n+1})^n\\&=\lim_{n\to\infty}(1-\frac{1}{n+1})^{n+1}*(\frac{n+1}{n})\\&=e^{-1}\end{aligned}$`  

例5.`$\lim_{x\to0}(\frac{1+\tan x}{1+\sin x})^\frac{1}{x^3}.$`  
> - `$1^\infty$`必定使用准则II。
> - `$\lim_{x\to a}f(x)=A\Rightarrow f(x)=A+\alpha$`

解：  
`$\begin{aligned}\lim_{x\to0}(\frac{1+\tan x}{1+\sin x})^\frac{1}{x^3}&=\lim_{x\to0}(1+\frac{\tan x-\sin x}{1+\sin x})^{\frac{1+\sin x}{\tan x-\sin x}*\frac{\tan x-\sin x}{1+\sin x}*\frac{1}{x^3}}\\&=e^{\lim_{x\to0}\frac{1}{1+\sin x}*\frac{\tan x-\sin x}{x^3}}\\&=e^{\frac{\tan x}{x}*\frac{1-\cos x}{x^2}}\\&=e^{\frac{1}{2}}\end{aligned}$`  